move implications into lemmas

src/SDK/Serialize/HeaderTypes.dfy
@@ -24,7 +24,13 @@ module HeaderTypes {
   | V1
   | V2
     {
-    function method Serialize(): (bytes: seq<uint8>)
+    function method Serialize(): (bytes: seq<uint8>) {
+      match this
+        case V1 => [0x01]
+        case V2 => [0x02]
+    }
+
+    lemma LemmaSerializeCorrectValue()
       //= compliance/data-format/message-header.txt#2.5.1.3
       //= type=implication
       //# The version (hex) of this field
@@ -34,17 +40,14 @@ module HeaderTypes {
         //= type=implication
         //# The value of the "Version" field MUST be "01" in the
         //# Version 1.0 header body.
-        case V1 => bytes == [0x01]
+        case V1 => this.Serialize() == [0x01]
         //= compliance/data-format/message-header.txt#2.5.1.2
         //= type=implication
         //# The value of the "Version" field MUST be "02" in the
         //# Version 2.0 header body.
-        case V2 => bytes == [0x02]
-    {
-      match this
-        case V1 => [0x01]
-        case V2 => [0x02]
-    }
+        case V2 => this.Serialize() == [0x02]
+    {}
+
     static function method Get(
       x: seq<uint8>
     )
@@ -59,6 +62,7 @@ module HeaderTypes {
       )
     }
   }
+
   datatype HeaderBody =
     | V1HeaderBody(
       nameonly messageType: MessageType,
@@ -89,16 +93,19 @@ module HeaderTypes {
   datatype MessageType =
   | TYPE_CUSTOMER_AED
     {
-    function method Serialize(): (val: uint8)
+    function method Serialize(): (val: uint8) {
+      match this
+      case TYPE_CUSTOMER_AED => 0x80
+    }
+
+    lemma LemmaSerializeCorrectValue()
       //= compliance/data-format/message-header.txt#2.5.1.4
       //= type=implication
       //# The type (hex) of this field MUST be
       //# a value that exists in the following table:
-      ensures val in {0x80}
-    {
-      match this
-      case TYPE_CUSTOMER_AED => 0x80
-    }
+      ensures this.Serialize() == 0x80
+    {}
+
     static function method Get(
       x: uint8
     )
@@ -117,18 +124,21 @@ module HeaderTypes {
   | NonFramed
   | Framed
   {
-    function method Serialize(): (val: uint8)
+    function method Serialize(): (val: uint8) {
+      match this
+      case NonFramed => 0x01
+      case Framed => 0x02
+    }
+
+    lemma LemmaSerializeCorrectValue()
       //= compliance/data-format/message-header.txt#2.5.1.11
       //= type=implication
       //# The value
       //# (hex) of this field MUST be a value that exists in the following
       //# table:
-      ensures val in {0x01, 0x02}
-    {
-      match this
-      case NonFramed => 0x01
-      case Framed => 0x02
-    }
+      ensures this.Serialize() in {0x01, 0x02}
+    {}
+
     static function method Get(
       x: uint8
     )
